maybe_relate_after_unfolding tac API

ocaml/fstar-lib/generated/FStar_Tactics_Basic.ml
@@ -7677,6 +7677,39 @@ let (refl_instantiate_implicits :
                            uu___9);
                     (e2, t1)))))
       else FStar_Tactics_Monad.ret FStar_Pervasives_Native.None
+let (refl_maybe_relate_after_unfolding :
+  env ->
+    FStar_Syntax_Syntax.term ->
+      FStar_Syntax_Syntax.term ->
+        FStar_TypeChecker_Core.side FStar_Pervasives_Native.option
+          FStar_Tactics_Monad.tac)
+  =
+  fun g ->
+    fun t0 ->
+      fun t1 ->
+        let uu___ =
+          ((no_uvars_in_g g) && (no_uvars_in_term t0)) &&
+            (no_uvars_in_term t1) in
+        if uu___
+        then
+          refl_typing_builtin_wrapper
+            (fun uu___1 ->
+               dbg_refl g
+                 (fun uu___3 ->
+                    let uu___4 = FStar_Syntax_Print.term_to_string t0 in
+                    let uu___5 = FStar_Syntax_Print.term_to_string t1 in
+                    FStar_Compiler_Util.format2
+                      "refl_maybe_relate_after_unfolding: %s and %s {\n"
+                      uu___4 uu___5);
+               (let s =
+                  FStar_TypeChecker_Core.maybe_relate_after_unfolding g t0 t1 in
+                dbg_refl g
+                  (fun uu___4 ->
+                     let uu___5 = FStar_TypeChecker_Core.side_to_string s in
+                     FStar_Compiler_Util.format1 "} returning side: %s\n"
+                       uu___5);
+                s))
+        else FStar_Tactics_Monad.ret FStar_Pervasives_Native.None
 let (tac_env : FStar_TypeChecker_Env.env -> FStar_TypeChecker_Env.env) =
   fun env1 ->
     let uu___ = FStar_TypeChecker_Env.clear_expected_typ env1 in
