src/tactics/FStar.Tactics.Embedding.fsti
@@ -21,6 +21,9 @@ open FStar.Syntax.Syntax
 open FStar.Syntax.Embeddings
 open FStar.Tactics.Types
 open FStar.Tactics.Result
+
+module Core = FStar.TypeChecker.Core
+
 module NBETerm = FStar.TypeChecker.NBETerm
 
 val e_exn                    : embedding exn
@@ -30,6 +33,7 @@ val e_result                 : embedding 'a -> embedding (__result 'a)
 val e_direction              : embedding direction
 val e_ctrl_flag              : embedding ctrl_flag
 val e_guard_policy           : embedding guard_policy
+val e_unfold_side            : embedding Core.side
 
 val e_exn_nbe                : NBETerm.embedding exn
 val e_proofstate_nbe         : NBETerm.embedding proofstate
@@ -38,6 +42,7 @@ val e_result_nbe             : NBETerm.embedding 'a -> NBETerm.embedding (__resu
 val e_direction_nbe          : NBETerm.embedding direction
 val e_ctrl_flag_nbe          : NBETerm.embedding ctrl_flag
 val e_guard_policy_nbe       : NBETerm.embedding guard_policy
+val e_unfold_side_nbe        : NBETerm.embedding Core.side
 
 val unfold_lazy_proofstate   : lazyinfo -> term
 val unfold_lazy_goal         : lazyinfo -> term
